Some progress but the correctness still need to be tuned

memabs/MemAbs.v
@@ -1,10 +1,11 @@
 Require Import Relations RelationClasses.
 Require Import List.
 Require Import Integers Coqlib Maps.
-Require Import LanguageInterface Events Globalenvs Values Memory AST Errors Smallstep.
-Require Import Clight Ctypes Cop.
+Require Import LanguageInterface Events Globalenvs Values Memory AST Errors Smallstep Linking.
+Require Import Clight Ctypes Cop SimplLocalsproof.
 Require Import CKLR Clightrel.
 Require Import Coherence CompCertSem Bigstep.
+Require Import SepCKLR.
 
 (* Define a language interface with memory abstracted out *)
 Record d_query :=
@@ -62,22 +63,23 @@ Next Obligation.
     f_equal. congruence. congruence.
 Defined.
 
-Section TRACE_STATE.
-  (* Since σ is not guaranteed to be a regular function, there is no way to "guess" the underlying
-     behavior w that corresponds to (qx, rx) *)
-  Program Definition next {liA liB: language_interface} (σ : !liA --o !liB) w qx rx : !liA --o !liB :=
-    {|
-    has '(s, t) := has σ (w ++ s, (qx, rx)::t);
-    |}.
-  Next Obligation.
-    intros liA liB sig w q r [s1 t1] [s2 t2] H1 H2 Ht.
-    pose proof (has_coh _ _ _ _ H1 H2). cbn in H. clear H1 H2.
-    edestruct H as [Hr Hl].
-    apply (@app_coh liA). apply Ht.
-    split. inversion Hr. subst. apply H5. auto.
-    intro. exploit Hl. f_equal. auto. apply app_inv_head.
-  Qed.
-End TRACE_STATE.
+Inductive exec {liA liB: language_interface} (σ: !liA --o !liB): query liB -> list (token liA) -> reply liB -> Prop:=
+| exec_intro: forall t q r,
+    has σ (t, (q, r) :: nil) ->
+    exec σ q t r.
+
+Program Definition next {liA liB: language_interface} (σ : !liA --o !liB) w qx rx : !liA --o !liB :=
+  {|
+  has '(s, t) := has σ (w ++ s, (qx, rx)::t);
+  |}.
+Next Obligation.
+  intros liA liB sig w q r [s1 t1] [s2 t2] H1 H2 Ht.
+  pose proof (has_coh _ _ _ _ H1 H2). cbn in H. clear H1 H2.
+  edestruct H as [Hr Hl].
+  apply (@app_coh liA). apply Ht.
+  split. inversion Hr. subst. apply H5. auto.
+  intro. exploit Hl. f_equal. auto. apply app_inv_head.
+Qed.
 
 Module Abs.
   Section ABS_SEMANTICS.
@@ -95,10 +97,12 @@ Module Abs.
     | step_internal: forall s s' t σ,
         Step (C se) s t s' ->
         step (st s σ) t (st s' σ)
-    | step_at_external: forall s s' qa ra qb rb σ w t,
+    | step_at_external: forall s s' qa ra qb rb σ w,
         Smallstep.at_external (C se) s qb ->
         Smallstep.after_external (C se) s rb s' ->
-        has (next σ w qa ra) t ->
+        (* (w, r) may not be the "right" execution. In other words, (next σ w q r) might be empty.
+           But that's fine because it's still related to s per correctness *)
+        exec σ qa w ra ->
         li_rel (qa, ra) (qb, rb) ->
         step (st s σ) E0 (ext s' w (next σ w qa ra))
     | step_after_external: forall s σ,
@@ -137,18 +141,18 @@ Module Abs.
     Smallstep.skel := skel;
     Smallstep.activate se := lts Σ C li_rel se;
     |}.
-  Definition c_semantics (C: Clight.program) (Σ: Genv.symtbl -> !li_d --o !li_d) : Smallstep.semantics li_d li_c :=
-    semantics (AST.erase_program C) li_rel Σ (semantics1 C).
+  Definition c_semantics sk (C: Clight.program) (Σ: Genv.symtbl -> !li_d --o !li_d) : Smallstep.semantics li_d li_c :=
+    semantics sk li_rel Σ (semantics1 C).
 End Abs.
 
 Module Impl.
   Section IMPL_SEMANTICS.
-    Context {liA liB: language_interface} (σ: Genv.symtbl -> !liB --o liA) (C: semantics liA liA).
+    Context {liA liB: language_interface} (σ: Genv.symtbl -> !liA --o liB) (C: semantics liB liB).
     Variable se: Genv.symtbl.
 
     Variant state :=
     | st (s: Smallstep.state C)
-    | ext (s: Smallstep.state C) (t: list (token liB)).
+    | ext (s: Smallstep.state C) (t: list (token liA)).
 
     Inductive step: state -> trace -> state -> Prop :=
     | step_internal: forall s s' t,
@@ -162,24 +166,24 @@ Module Impl.
     | step_after_external: forall s,
         step (ext s nil) E0 (st s).
 
-    Inductive initial_state: query liA -> state -> Prop :=
+    Inductive initial_state: query liB -> state -> Prop :=
     | initial_state_intro: forall q s,
         Smallstep.initial_state (C se) q s ->
         initial_state q (st s).
 
-    Inductive at_external: state -> query liB -> Prop :=
+    Inductive at_external: state -> query liA -> Prop :=
     | ext_at_external: forall s q r t,
         at_external (ext s ((q, r) :: t)) q.
-    Inductive after_external: state -> reply liB -> state -> Prop :=
+    Inductive after_external: state -> reply liA -> state -> Prop :=
     | ext_after_external: forall s q r t,
         after_external (ext s ((q, r) :: t)) r (ext s t).
 
-    Inductive final_state: state -> reply liA -> Prop :=
+    Inductive final_state: state -> reply liB -> Prop :=
     | final_state_intro: forall s r,
         Smallstep.final_state (C se) s r ->
         final_state (st s) r.
 
-    Definition lts : lts liB liA state :=
+    Definition lts : lts liA liB state :=
       {|
       Smallstep.step _ := step;
       Smallstep.valid_query := Smallstep.valid_query (C se);
@@ -195,62 +199,143 @@ Module Impl.
     Smallstep.skel := skel;
     Smallstep.activate se := lts σ C se;
     |}.
-  Definition c_semantics (C: Clight.program) (p: Clight.program): Smallstep.semantics li_d li_c :=
-    semantics (AST.erase_program C) (fun se => clight_bigstep p se @ !li_dc) (semantics1 C).
+  Definition c_semantics sk (C: Clight.program) (p: Clight.program): Smallstep.semantics li_d li_c :=
+    semantics sk (fun se => clight_bigstep p se @ !li_dc) (semantics1 C).
 End Impl.
 
-Section CORRECT.
-  Inductive module_var (ge: genv) : block -> Z -> Prop :=
-  | module_var_intro id b (v : globvar type) (ty : type):
-      Genv.find_symbol ge id = Some b ->
-      Genv.find_def ge b = Some (Gvar v) ->
-      ty = gvar_info v ->
-      module_var ge b (sizeof ge ty).
-  Definition non_module_var ge b ofs := ~ module_var ge b ofs.
-  Variable p: Clight.program.
-  Variable se: Genv.symtbl.
-  Let clight_p: !li_c --o li_c := clight_bigstep p se. (* the semantics of the clight program *)
-  (* the semantics of the clight program on top of a deepsea underlay *)
-  Let d_p : !li_d --o li_c := clight_p @ !li_dc.
-  (* the coherent space where specification lives in *)
-  Let spec_space : space := !li_d --o !li_d.
-  (* the specification *)
-  Variable spec : !li_d --o !li_d.
+Inductive module_var (ge: genv) : block -> Z -> Prop :=
+| module_var_intro id b (v : globvar type) (ty : type):
+    Genv.find_symbol ge id = Some b ->
+    Genv.find_def ge b = Some (Gvar v) ->
+    ty = gvar_info v ->
+    module_var ge b (sizeof ge ty).
 
-  Record correctness :=
-    {
-    (* rel : the relation that relates specifications and the memory *)
-    rel :> token spec_space -> mem -> Prop;
-    (* the condition that the memory has to satisfy *)
-    init_mem : mem -> Prop;
-    mem_scope : forall m m' t, Mem.unchanged_on (module_var (Clight.globalenv se p)) m m' -> rel t m -> rel t m';
-    simulation:
-      forall s dq dr t m,
-        rel (s, (dq, dr)::t) m ->
-        exists u v cr cq m',
-          s = u ++ v /\
-          (* Clight implementation simulates deepsea event e *)
-          q_rel dq cq m /\
-          has d_p (u, (cq, cr)) /\
-          r_rel dr cr m' /\
-          Mem.unchanged_on (non_module_var (Clight.globalenv se p)) m m' /\
-          (* behavior of the remaning trace *)
-          rel (v, t) m';
-    correct_cond: forall m t, has spec t -> init_mem m -> rel t m;
-    }.
-End CORRECT.
+Record prog_sim (p: Clight.program) (Σ: Genv.symtbl -> !li_d --o !li_d) :=
+  {
+  mspec_rel :> (!li_d --o !li_d) -> mem -> Prop;
+  init_mem : mem -> Prop;
+
+  mem_scope : forall m m' σ se,
+      Genv.valid_for (AST.erase_program p) se ->
+      Mem.unchanged_on (module_var (Clight.globalenv se p)) m m' ->
+      mspec_rel σ m ->
+      mspec_rel σ m';
+  simulation: forall σ dq dr t m se,
+      Genv.valid_for (AST.erase_program p) se ->
+      mspec_rel σ m -> exec σ dq t dr ->
+      exists cr cq m',
+        q_rel dq cq m /\ r_rel dr cr m' /\
+        has (clight_bigstep p se @ !li_dc) (t, (cq, cr)) /\
+        Mem.unchanged_on (fun b ofs => ~ module_var (Clight.globalenv se p) b ofs) m m' /\
+        mspec_rel (next σ t dq dr) m';
+  correct_cond: forall m se,
+      Genv.valid_for (AST.erase_program p) se ->
+      init_mem m -> mspec_rel (Σ se) m;
+  }.
+
+Definition get_mem (s: state) : mem :=
+  match s with
+  | State _ _ _ _ _ m => m
+  | Callstate _ _ _ m => m
+  | Returnstate _ _ m => m
+  end.
 
 Section SIM.
-  Context {p: Clight.program} {se: Genv.symtbl} {Σ: Genv.symtbl -> !li_d --o !li_d}
-          (correct: correctness p se (Σ se)).
+  Context {p: Clight.program} {Σ: Genv.symtbl -> !li_d --o !li_d} (ps: prog_sim p Σ).
   Variable C: Clight.program.
-  Definition sem_abs: semantics li_d li_c := Abs.c_semantics C Σ.
-  Definition sem_impl: semantics li_d li_c := Impl.c_semantics C p.
+  Context {sk: AST.program unit unit} (Hlk: link (skel (semantics1 C)) (skel (semantics1 p)) = Some sk).
+  Definition sem_abs: semantics li_d li_c := Abs.c_semantics sk C Σ.
+  Definition sem_impl: semantics li_d li_c := Impl.c_semantics sk C p.
 
-  Inductive state_match: Smallstep.state sem_abs -> Smallstep.state sem_impl -> Prop := .
+  (* It's not possible to infer the outgoing interface so we define the following notations *)
+  Notation " 'st1' " := (@Abs.st li_d li_c (semantics1 C)) (at level 1) : sim_scope.
+  Notation " 'st2' " := (@Impl.st li_d li_c (semantics1 C)) (at level 1) : sim_scope.
+  Notation " 'ext1' " := (@Abs.ext li_d li_c (semantics1 C)) (at level 1) : sim_scope.
+  Notation " 'ext2' " := (@Impl.ext li_d li_c (semantics1 C)) (at level 1) : sim_scope.
+  Notation " 'state1' " := (@Abs.state li_d li_c (semantics1 C)) (at level 1) : sim_scope.
+  Notation " 'state2' " := (@Impl.state li_d li_c (semantics1 C)) (at level 1) : sim_scope.
+  Open Scope sim_scope.
 
-  Variable R: cklr.             (* this will be instantiated to the cklr defined below *)
+  Section MATCH.
+    Inductive state_match {ind} (ms: ind -> state -> state -> Prop): state1 -> state2 -> Prop :=
+    | st_match: forall (s1 s2: state) σ1 i,
+        ms i s1 s2 ->  ps σ1 (get_mem s2)->
+        state_match ms (st1 s1 σ1) (st2 s2)
+    | ext_match: forall (s1 s2: state) σ1 t1 t2 i,
+        ms i s1 s2 -> t1 = t2 ->
+        ps σ1 (get_mem s2)->
+        state_match ms (ext1 s1 t1 σ1) (ext2 s2 t2).
+  End MATCH.
+  Variable se: Genv.symtbl.
+  Let vars := module_var (Clight.globalenv se p).
+  Let sepv := sep vars.
+  Instance sepv_frame: KripkeFrame unit (sep_world vars).
+  Proof. exact (cklr_kf sepv). Qed.
+
   Theorem fsim_abs_impl:
-    forward_simulation cc_id (cc_c R) sem_abs sem_impl.
+    forward_simulation cc_id (cc_c sepv) sem_abs sem_impl.
+  Proof.
+    pose proof (semantics1_rel C sepv) as [[ind ord match_st _ H _]].
+    constructor. econstructor; eauto. instantiate (1 := fun _ _ _ => _). cbn beta.
+    intros se1 se2 w Hse Hse1. cbn -[sem_abs sem_impl semantics1] in *.
+    eapply link_linkorder in Hlk as [HseC Hsep].
+    eapply Genv.valid_for_linkorder in HseC; eauto.
+    eapply Genv.valid_for_linkorder in Hsep; eauto.
+    specialize (H se1 se2 w Hse HseC).
+    assert (se = se1). admit. subst se2. subst se1.
+    (* apply forward_simulation_step with *)
+    (*     (match_states := fun s1 s2 => klr_diam tt (state_match (match_st se se)) w s1 s2). *)
+    apply forward_simulation_step with (match_states := (state_match (match_st se se w))).
+    - intros. exploit @fsim_match_valid_query; eauto.
+    - cbn. intros q1 q2 s1 Hq Hs1.
+      cbn in Hs1. inv Hs1.
+      edestruct @fsim_match_initial_states as (i & s2 & Hiq & Hs); eauto.
+      exists(st2 s2). split. constructor. auto.
+      eapply st_match. apply Hs. eapply correct_cond. auto. admit.
+    (* initial query has to satisfy init_mem. Maybe we have to parametrize the
+       semantics over some proposition on memory *)
+    - admit.
+    - admit.
+    - intros s1 t s1' Hstep s2 Hs. inversion Hstep.
+      + admit.
+      + subst. cbn. inv Hs.
+        edestruct @fsim_match_external as (w' & qtgt & Hext & mq & msenv & fsim_match_after_ext); eauto.
+        edestruct (simulation _ _ ps) as (rb' & qtgt' & m' & qrel & rrel & impl & mem_unchange & Hs'); eauto.
+        assert (cc_c_reply sepv w' rb rb').
+        {
+          unfold sepv. destruct rb as [vres_src m_src]. destruct rb' as [vres_tgt m_tgt].
+          constructor.
+          - inv H3. inv rrel.
+            apply val_inject_refl.
+          - cbn. destruct w'. econstructor.
+            + admit.            (* memory extension might not hold after external calls *)
+            + admit.
+            + admit.
+        }
+        edestruct fsim_match_after_ext as (i' & s2' & Haft & Hs2); eauto. exists w'. split. admit.
+        eauto.
+        exists(ext2 s2' w0). split.
+        * econstructor. apply Hext. apply Haft.
+          assert (qtgt = qtgt').
+          {
+            destruct qtgt as [vf0 sg0 args0 m0].
+            destruct qtgt' as [vf1 sg1 args1 m1].
+            inv qrel. inv Hext. inv H3. inv mq. f_equal.
+            cbn in H12. SearchAbout Val.inject inject_id.
+            rewrite val_inject_id in H12. inv H12. auto.
+            congruence.
+            admit.              (* Vundef args *)
+          }
+          rewrite H5. apply impl.
+        * econstructor. apply Hs2. auto.
+          assert (m' = get_mem s2').
+          {
+            inv Haft. inv rrel. auto.
+          }
+          rewrite <- H5. apply Hs'.
+      + admit.
+    - admit.
   Admitted.
+
+  Close Scope sim_scope.
 End SIM.
